wip

crypto_hst/ec/Hacl.EC.Curve25519.Bignum.Fdifference.Lemmas.fst
@@ -4,12 +4,15 @@ open FStar.Mul
 open FStar.HST
 open FStar.HyperStack
 open FStar.Ghost
-open Hacl.UInt64
-open Hacl.SBuffer
+open FStar.Buffer
 open FStar.Math.Lib
+open FStar.Math.Lemmas
+
+open Hacl.UInt64
+
 open Hacl.EC.Curve25519.Parameters
 open Hacl.EC.Curve25519.Bigint
-
+open Hacl.EC.Curve25519.Bignum.Lemmas.Utils
 
 #reset-options "--initial_fuel 0 --max_fuel 0"
 
@@ -23,316 +26,352 @@ module H8  = Hacl.UInt8
 module H32  = Hacl.UInt32
 module H64  = Hacl.UInt64
 
-#set-options "--lax"
+let addedZero h0 h1 (b:bigint) : GTot Type0 =
+  norm h0 b /\ live h1 b
+  /\ v (get h1 b 0) = v (get h0 b 0) + (pow2 52 - 38)
+  /\ v (get h1 b 1) = v (get h0 b 1) + (pow2 52 - 2)
+  /\ v (get h1 b 2) = v (get h0 b 2) + (pow2 52 - 2)
+  /\ v (get h1 b 3) = v (get h0 b 3) + (pow2 52 - 2)
+  /\ v (get h1 b 4) = v (get h0 b 4) + (pow2 52 - 2)
 
-module U32 = FStar.UInt32
+val lemma_pow2_52m38: unit -> Lemma (0xfffffffffffda = pow2 52 - 38)
+let lemma_pow2_52m38 () = assert_norm(0xfffffffffffda = pow2 52 - 38)
 
-let op_Plus_Bar = U32.add
-let op_Subtraction_Bar = U32.sub
+val lemma_pow2_52m2: unit -> Lemma (0xffffffffffffe = pow2 52 - 2)
+let lemma_pow2_52m2 () = assert_norm(0xffffffffffffe = pow2 52 - 2)
 
-val helper_lemma_1:
-  i:nat -> len:nat -> x:nat -> 
-  Lemma (requires (i < len /\ len <= x)) (ensures (i < x))
-let helper_lemma_1 i len v = ()  
-
-(* #reset-options *)
-val fdifference_aux_1: a:bigint -> b:bigint{disjoint a b} -> ctr:u32{U32.v ctr < norm_length} -> STL unit
-    (requires (fun h -> live h a /\ live h b /\ norm_length <= length a /\ norm_length <= length b
-              /\ (forall (i:nat{ i >= U32.v ctr /\ i < norm_length}). v (get h b i) >= v (get h a i))))
-    (ensures (fun h0 _ h1 -> 
-      live h0 a /\ live h1 a /\ live h0 b /\ live h1 b
-      /\ length a = length a /\ length b = length b
-      /\ norm_length <= length a /\ norm_length <= length b /\ modifies_1 a h0 h1
-      /\ (forall (i:nat).
-	((i >= U32.v ctr+1 /\ i < norm_length) ==>  (v (get h1 b i) >= v (get h1 a i)
-						/\ get h1 a i == get h0 a i))
-	/\ (((i<U32.v ctr \/ i>=norm_length) /\ i<length a) ==> get h1 a i == get h0 a i))
-      /\ v (get h1 a (U32.v ctr)) = v (get h0 b (U32.v ctr)) - v (get h0 a (U32.v ctr))))
-
-let fdifference_aux_1 a b ctr =
-  //@@
-  let h0 = HST.get() in
-  let i = ctr in
-  (* FdifferenceLemmas.helper_lemma_3 i norm_length;  *)
-  helper_lemma_1 (U32.v i) norm_length (length a);
-  helper_lemma_1 (U32.v i) norm_length (length b);
-  let ai = index a i in 
-  let bi = index b i in 
-  assert(U32.v i >= U32.v ctr /\ U32.v i < norm_length); 
-  cut(b2t(v (get h0 b (U32.v i)) >= v (get h0 a (U32.v i)))); 
-  let z = bi -^ ai in 
-  upd a i z;
-  let h1 = HST.get() in
-  (* upd_lemma h0 h1 a i z; *)
-  (* no_upd_lemma h0 h1 b ((only a)) *)
-  ()
-  
-val fdifference_aux_2_0: h0:heap -> h1:heap -> h2:heap -> a:bigint -> b:bigint{disjoint a b} -> 
-  ctr:nat{ctr < norm_length} -> Lemma (requires (
-      live h0 a /\ live h1 a /\ live h2 a /\ live h0 b /\ live h1 b /\ live h2 b
-      /\ modifies_1 a h0 h1 /\ modifies_1 a h1 h2
-      // Conditions from fdifference_aux
-      /\ (modifies_1 a h1 h2)
-      /\ (forall (i:nat).
-	  ((i>=ctr+1 /\ i<norm_length) ==> (v (get h2 a i) = v (get h1 b i) - v (get h1 a i)))
-	  /\ (((i<ctr+1 \/ i >= norm_length) /\ i<length a) ==> (get h2 a i == get h1 a i)))
-      // Conditions from fdifference_aux_1
-      /\ (forall (i:nat).
-	  ((i >= ctr+1 /\ i < norm_length) ==>
-	    v (get h1 b i) >= v (get h1 a i) /\ get h1 a i == get h0 a i)
-	  /\ (((i<ctr \/ i >= norm_length) /\ i<length a) ==> get h1 a i == get h0 a i))
-      /\ v (get h1 a ctr) = v (get h0 b ctr) - v (get h0 a ctr)))
-    (ensures (
-      (live h0 a) /\ (live h0 b) /\ (live h2 a) /\ (live h2 b)
-      /\ (modifies_1 a h0 h2)
-      /\ (length a = length a)
-      /\ (forall (i:nat). (i>= ctr /\ i<norm_length) ==> (v (get h2 a i) = v (get h0 b i) - v (get h0 a i)))
-      ))
-      
-let fdifference_aux_2_0 h0 h1 h2 a b ctr =
-  //@@
-  (* no_upd_lemma h0 h1 b ((only a)); *)
-  assert(length a = length a);
-  assert(forall (i:nat). (i>= ctr+1 /\ i<norm_length) ==>
-	  (v (get h2 a i) = v (get h1 b i) - v (get h1 a i)));  
-  assert(forall (i:nat). (i>=ctr+1 /\ i < norm_length) ==> get h1 a i == get h0 a i); 
-  assert(get h2 a ctr == get h1 a ctr); 
-  assert(v (get h1 a ctr) = v (get h0 b ctr) - v (get h0 a ctr));
-  cut(forall (i:nat). (i>= ctr+1 /\ i<norm_length) ==>
-	  (v (get h2 a i) = v (get h0 b i) - v (get h0 a i))); 
-  cut(True /\ v (get h2 a ctr) = v (get h0 b ctr) - v (get h0 a ctr)); 
-  (* FdifferenceLemmas.helper_lemma_5 ctr norm_length; *)
-  assert(forall (i:nat). (i>=ctr /\ i < norm_length) ==>
-	   (v (get h2 a i) = v (get h0 b i) - v (get h0 a i)))
-
-(* #reset-options *)
-
-val fdifference_aux_2_1: h0:heap -> h1:heap -> h2:heap -> a:bigint -> b:bigint{disjoint a b} -> 
-  ctr:nat{ctr < norm_length} ->
+val lemma_add_big_zero_core:
+  b0:H64.t -> b1:H64.t -> b2:H64.t -> b3:H64.t -> b4:H64.t ->
   Lemma 
-    (requires (
-      live h0 a /\ live h1 a /\ live h2 a /\ live h0 b /\ live h1 b /\ live h2 b
-      /\ modifies_1 a h0 h1 /\ modifies_1 a h1 h2
-      /\ length a = length a /\ length a = length a
-      /\ length b = length b /\ length b = length b
-      /\ (norm_length <= length a /\ norm_length <= length b)
-      // Conditions from fdifference_aux
-      /\ (modifies_1 a h1 h2)
-      /\ (forall (i:nat).
-	  ((i>=ctr+1 /\ i<norm_length) ==> (v (get h2 a i) = v (get h1 b i) - v (get h1 a i)))
-	  /\ (((i<ctr+1 \/ i >= norm_length) /\ i<length a) ==> (get h2 a i == get h1 a i)))
-      // Conditions from fdifference_aux_1
-      /\ (forall (i:nat).
-	  ((i >= ctr+1 /\ i < norm_length) ==>
-	    v (get h1 b i) >= v (get h1 a i) /\ get h1 a i == get h0 a i)
-	  /\ (((i<ctr \/ i >= norm_length) /\ i<length a) ==> get h1 a i == get h0 a i))
-      /\ v (get h1 a ctr) = v (get h0 b ctr) - v (get h0 a ctr)))
-    (ensures (
-      (live h0 a) /\ (live h0 b) /\ (live h2 a) /\ (live h2 b)
-      /\ (norm_length <= length a /\ norm_length <= length b)
-      /\ (modifies_1 a h0 h2)
-      /\ (length a = length a)
-      /\ (forall (i:nat). ((i<ctr \/ i >= norm_length) /\ i<length a) ==> (get h2 a i == get h0 a i))
-    ))
-let fdifference_aux_2_1 h0 h1 h2 a b ctr = 
-  //@@
-  ()
+    (requires (v b0 < pow2 51 /\ v b1 < pow2 51 /\ v b2 < pow2 51 /\ v b3 < pow2 51 /\ v b4 < pow2 51))
+    (ensures  (v b0 + pow2 52 - 38 < pow2 64
+      /\ v b1 + pow2 52 - 2 < pow2 64
+      /\ v b2 + pow2 52 - 2 < pow2 64
+      /\ v b3 + pow2 52 - 2 < pow2 64
+      /\ v b4 + pow2 52 - 2 < pow2 64))
+let lemma_add_big_zero_core b0 b1 b2 b3 b4 =
+  assert_norm(pow2 1 = 2);
+  pow2_lt_compat 52 1;
+  pow2_double_sum 51;
+  pow2_double_sum 52;
+  pow2_lt_compat 64 53
 
-val fdifference_aux_2: h0:heap -> h1:heap -> h2:heap -> a:bigint -> b:bigint{disjoint a b} -> 
-  ctr:nat{ctr < norm_length} -> Lemma
-    (requires (
-      live h0 a /\ live h1 a /\ live h2 a /\ live h0 b /\ live h1 b /\ live h2 b
-      /\ modifies_1 a h0 h1 /\ modifies_1 a h1 h2
-      /\ length a = length a /\ length a = length a
-      /\ length b = length b /\ length b = length b
-      /\ (norm_length <= length a /\ norm_length <= length b)
-      // Conditions from fdifference_aux
-      /\ (modifies_1 a h1 h2)
-      /\ (forall (i:nat). 
-	  ((i>= ctr+1 /\ i<norm_length) ==>
-	    (v (get h2 a i) = v (get h1 b i) - v (get h1 a i)))
-	  /\ (((i<ctr+1 \/ i >= norm_length) /\ i<length a) ==> (get h2 a i == get h1 a i)))
-      // Conditions from fdifference_aux_1
-      /\ (forall (i:nat).
-	  ((i >= ctr+1 /\ i < norm_length) ==> v (get h1 b i) >= v (get h1 a i)
-						/\ get h1 a i == get h0 a i)
-	  /\ (((i<ctr \/ i >= norm_length) /\ i<length a) ==> get h1 a i == get h0 a i))
-      /\ v (get h1 a ctr) = v (get h0 b ctr) - v (get h0 a ctr)))
-    (ensures (
-      (live h0 a) /\ (live h0 b) /\ (live h2 a) /\ (live h2 b)
-      /\ (norm_length <= length a /\ norm_length <= length b)
-      /\ (modifies_1 a h0 h2)
-      /\ (length a = length a)
-      /\ (forall (i:nat).
-	  ((i>= ctr /\ i<norm_length) ==> 
-	    (v (get h2 a i) = v (get h0 b i) - v (get h0 a i)))
-	  /\ (((i<ctr \/ i >= norm_length) /\ i<length a) ==> (get h2 a i == get h0 a i)))
-      ))      
-let fdifference_aux_2 h0 h1 h2 a b ctr =
-  //@@
-  fdifference_aux_2_0 h0 h1 h2 a b ctr;
-  fdifference_aux_2_1 h0 h1 h2 a b ctr
+let bound53 h (b:bigint) : GTot Type0 =
+  live h b
+  /\ v (get h b 0) < pow2 53
+  /\ v (get h b 1) < pow2 53
+  /\ v (get h b 2) < pow2 53
+  /\ v (get h b 3) < pow2 53
+  /\ v (get h b 4) < pow2 53
 
-(* #reset-options *)
+(* module U32 = FStar.UInt32 *)
 
-val fdifference_aux: a:bigint -> b:bigint{disjoint a b} -> ctr:u32{U32.v ctr <= norm_length } -> STL unit
-    (requires (fun h -> live h a /\ live h b
-      /\ (forall (i:nat). (i >= U32.v ctr /\ i < norm_length) ==> (v (get h b i) >= v (get h a i))) ))
-    (ensures (fun h0 _ h1 -> 
-      (live h0 a) /\ (live h0 b) /\ (live h1 a) /\ (live h1 b)
-      /\ (norm_length <= length a /\ norm_length <= length b)
-      /\ (modifies_1 a h0 h1)
-      /\ (length a = length a)
-      /\ (forall (i:nat). 
-	  ((i>= U32.v ctr /\ i<norm_length) ==>  
-	    (v (get h1 a i) = v (get h0 b i) - v (get h0 a i)))
-	  /\ (((i<U32.v ctr \/ i >= norm_length) /\ i<length a) ==> (get h1 a i == get h0 a i)))
-    ))
-let rec fdifference_aux a b ctr =
-  //@@
-  let h0 = HST.get() in
-  if U32.eq ctr nlength then ()
-  else begin
-      fdifference_aux_1 a b ctr; 
-      let h1 = HST.get() in
-      (* no_upd_lemma h0 h1 b ((only a)); *)
-      fdifference_aux a b (ctr+|1ul); 
-      let h2 = HST.get() in
-      fdifference_aux_2 h0 h1 h2 a b (U32.v ctr)
-  end
-  
-(* #reset-options *)
+(* let op_Plus_Bar = U32.add *)
+(* let op_Subtraction_Bar = U32.sub *)
 
-val subtraction_lemma_aux: h0:heap ->  h1:heap -> a:bigint{live h0 a /\ live h1 a} -> 
-  b:bigint{live h0 b} -> len:pos{len <= length a /\ len <= length b
-    /\ (forall (i:nat). i < len ==> v (get h1 a i) = v (get h0 b i) - v (get h0 a i)) } ->
-  Lemma (requires ( (eval h0 b (len-1) - eval h0 a (len-1) = eval h1 a (len-1))
-		/\ (v (get h1 a (len-1)) = v (get h0 b (len-1)) - v (get h0 a (len-1))) ) )
-    (ensures (eval h0 b len - eval h0 a len = eval h1 a len))
-let subtraction_lemma_aux h0 h1 a b len =
-  //@@
-  eval_def h1 a len;
-  assert(eval h1 a len = pow2 (bitweight (templ) (len-1)) * v (get h1 a (len-1)) + eval h1 a (len-1));
-  assert(v (get h1 a (len-1)) = v (get h0 b (len-1)) - v (get h0 a (len-1))); 
-  Math.Axioms.distributivity_sub_right (pow2 (bitweight (templ) (len-1))) (v (get h0 b (len-1)))  (v (get h0 a (len-1))); 
-  assert(eval h1 a len = (pow2 (bitweight (templ) (len-1)) * v (get h0 b (len-1)) - pow2 (bitweight (templ) (len-1)) * v (get h0 a (len-1))) + eval h1 a (len-1));
-  (* FdifferenceLemmas.helper_lemma_2  *)
-  (* 		(pow2 (bitweight (templ) (len-1)) * v (get h0 b (len-1))) *)
-  (* 		(pow2 (bitweight (templ) (len-1)) * v (get h0 a (len-1))) *)
-  (* 		(eval h0 b (len-1)) *)
-  (* 		(eval h0 a (len-1)); *)
-  eval_def h0 a len;
-  eval_def h0 b len
+(* val helper_lemma_1: *)
+(*   i:nat -> len:nat -> x:nat ->  *)
+(*   Lemma (requires (i < len /\ len <= x)) (ensures (i < x)) *)
+(* let helper_lemma_1 i len v = ()   *)
 
-(* #reset-options *)
+(* (\* #reset-options *\) *)
+(* val fdifference_aux_1: a:bigint -> b:bigint{disjoint a b} -> ctr:u32{U32.v ctr < norm_length} -> STL unit *)
+(*     (requires (fun h -> live h a /\ live h b /\ norm_length <= length a /\ norm_length <= length b *)
+(*               /\ (forall (i:nat{ i >= U32.v ctr /\ i < norm_length}). v (get h b i) >= v (get h a i)))) *)
+(*     (ensures (fun h0 _ h1 ->  *)
+(*       live h0 a /\ live h1 a /\ live h0 b /\ live h1 b *)
+(*       /\ length a = length a /\ length b = length b *)
+(*       /\ norm_length <= length a /\ norm_length <= length b /\ modifies_1 a h0 h1 *)
+(*       /\ (forall (i:nat). *)
+(* 	((i >= U32.v ctr+1 /\ i < norm_length) ==>  (v (get h1 b i) >= v (get h1 a i) *)
+(* 						/\ get h1 a i == get h0 a i)) *)
+(* 	/\ (((i<U32.v ctr \/ i>=norm_length) /\ i<length a) ==> get h1 a i == get h0 a i)) *)
+(*       /\ v (get h1 a (U32.v ctr)) = v (get h0 b (U32.v ctr)) - v (get h0 a (U32.v ctr)))) *)
 
-val subtraction_lemma:
-  h0:heap -> h1:heap -> a:bigint{live h0 a /\ live h1 a} -> b:bigint{live h0 b} ->
-  len:nat{len <= length a /\ len <= length b
-  /\ (forall (i:nat). i < len ==> v (get h1 a i) = v (get h0 b i) - v (get h0 a i)) } -> Lemma
-    (requires (True))
-    (ensures ( eval h0 b len - eval h0 a len = eval h1 a len ))
-let rec subtraction_lemma h0 h1 a b len =
-  //@@
-  match len with
-  | 0 -> ()
-  | _ -> subtraction_lemma h0 h1 a b (len-1);
-    subtraction_lemma_aux h0 h1 a b len
-
-(* #reset-options *)
-
-val subtraction_max_value_lemma: h0:heap -> h1:heap -> a:bigint{live h0 a} -> 
-  b:bigint{live h0 b /\ length a = length b} ->
-  c:bigint{live h1 c /\ length c = length a
-   /\ (forall (i:nat). (i<length c) ==> v (get h1 c i) = v (get h0 b i) - v (get h0 a i)) } ->
-  Lemma
-    (requires (True))
-    (ensures (maxValue h1 c (length c) <= maxValue h0 b (length c)))
-let subtraction_max_value_lemma h0 h1 a b c = 
-  //@@
-  ()
-
-(* #reset-options *)
-
-val max_value_lemma: h:heap -> a:bigint{live h a} -> m:nat ->Lemma 
-    (requires (forall (n:nat). n < length a ==> v (get h a n) <= m))
-    (ensures (maxValue h a (length a) <= m))
-let max_value_lemma h a m = 
-  //@@
-  ()
-
-val subtraction_max_value_lemma_extended: h0:heap -> h1:heap -> a:bigint{live h0 a} -> 
-  b:bigint{live h0 b} ->
-  c:bigint{live h1 c /\ length a = length c} -> 
-  Lemma
-    (requires ((forall (i:nat). (i<norm_length) ==> 
-		  v (get h1 c i) = v (get h0 b i) - v (get h0 a i))
-	       /\ (forall (i:nat). (i < length c /\ i >= norm_length) ==>
-		   v (get h1 c i) = v (get h0 a i))))
-    (ensures (maxValue h1 c (length c) <= max (maxValue h0 a (length a)) (maxValue h0 b (length b))))
-let subtraction_max_value_lemma_extended h0 h1 a b c = 
-  //@@
-  cut ( forall (i:nat). (i < length c /\ i >= norm_length)
-	==> (v (get h1 c i) = v (get h0 a i) /\ v (get h1 c i) <= maxValue h0 a (length a)));
-  cut ( forall (i:nat). (i < length c /\ i >= norm_length)
-  	==> v (get h1 c i) <= max (maxValue h0 a (length a)) (maxValue h0 b (length b)));	
-  assert ( forall (i:nat). (i < norm_length)
-	==> v (get h1 c i) = v (get h0 b i) - v (get h0 a i));
-  (* assert(forall (i:nat). (i < norm_length) ==> v (get h1 c i) = v (get h0 b i) - v (get h0 a i) ==> v (get h1 c i) <= v (get h0 b i) ==> v (get h1 c i) <= maxValue h0 b);  *)
-  (* cut ( forall (i:nat). (i < norm_length) *)
-  (* 	==> v (get h1 c i) <= maxValue h0 b);  *)
-  (* cut ( forall (i:nat). (i < norm_length) *)
-  (* 	==> (v (get h0 a i) <= maxValue h0 a /\ v (get h0 b i) <= maxValue h0 b));  *)
-  cut ( forall (i:nat). (i < norm_length)
-	==> v (get h1 c i) <= max (maxValue h0 a (length a)) (maxValue h0 b (length b)))
-
-(* #reset-options *)
-
-val auxiliary_lemma_2: ha:heap -> a:bigint{norm ha a} -> hb:heap -> b:bigint{filled hb b} -> 
-  i:nat{i < norm_length} -> Lemma (v (get hb b i) - v (get ha a i) < pow2 (templ i + 1))
-let auxiliary_lemma_2 ha a hb b i = ()
-  //@@
-  (* assert(True /\ bitsize (v (get hb b i)) max);  *)
-  (* Lemmas.pow2_increases_2 min (templ i);  *)
-  (* assert(bitsize (v (get ha a i)) (templ i));  *)
-  (* assert(v (get ha a i) < pow2 (templ i));  *)
-  (* cut(True /\ v (get ha a i) < pow2 min);  *)
-  (* assert(bitsize (v (get ha a i)) min);  *)
-  (* UInt.sub_lemma #max (v (get hb b i)) (v (get ha a i)) *)
-
-(* #reset-options *)
-
-val auxiliary_lemma_0: ha:heap -> a:bigint{norm ha a} -> hb:heap -> b:bigint{filled hb b} ->
-  Lemma (forall (i:nat). i < norm_length ==> v (get hb b i) - v (get ha a i) < pow2 (templ i + 1))
-let auxiliary_lemma_0 ha a hb b = 
-  //@@
-  ()
-
-(* #reset-options *)
-
-(* val auxiliary_lemma_1: h0:heap -> h1:heap -> mods:FStar.Set.set abuffer -> b:bigint{filled h0 b} -> *)
-(*   Lemma (requires (live h1 b /\ modifies mods h0 h1 /\ not(FStar.Set.mem (Ref (getRef b)) mods))) *)
-(* 	(ensures (filled h1 b)) *)
-(* let auxiliary_lemma_1 h0 h1 mods min max b =  *)
+(* let fdifference_aux_1 a b ctr = *)
 (*   //@@ *)
-(*   assert(FStar.Seq.Eq (sel h0 (getRef b)) (sel h1 (getRef b)));  *)
+(*   let h0 = HST.get() in *)
+(*   let i = ctr in *)
+(*   (\* FdifferenceLemmas.helper_lemma_3 i norm_length;  *\) *)
+(*   helper_lemma_1 (U32.v i) norm_length (length a); *)
+(*   helper_lemma_1 (U32.v i) norm_length (length b); *)
+(*   let ai = index a i in  *)
+(*   let bi = index b i in  *)
+(*   assert(U32.v i >= U32.v ctr /\ U32.v i < norm_length);  *)
+(*   cut(b2t(v (get h0 b (U32.v i)) >= v (get h0 a (U32.v i))));  *)
+(*   let z = bi -^ ai in  *)
+(*   upd a i z; *)
+(*   let h1 = HST.get() in *)
+(*   (\* upd_lemma h0 h1 a i z; *\) *)
+(*   (\* no_upd_lemma h0 h1 b ((only a)) *\) *)
+(*   () *)
+  
+(* val fdifference_aux_2_0: h0:heap -> h1:heap -> h2:heap -> a:bigint -> b:bigint{disjoint a b} ->  *)
+(*   ctr:nat{ctr < norm_length} -> Lemma (requires ( *)
+(*       live h0 a /\ live h1 a /\ live h2 a /\ live h0 b /\ live h1 b /\ live h2 b *)
+(*       /\ modifies_1 a h0 h1 /\ modifies_1 a h1 h2 *)
+(*       // Conditions from fdifference_aux *)
+(*       /\ (modifies_1 a h1 h2) *)
+(*       /\ (forall (i:nat). *)
+(* 	  ((i>=ctr+1 /\ i<norm_length) ==> (v (get h2 a i) = v (get h1 b i) - v (get h1 a i))) *)
+(* 	  /\ (((i<ctr+1 \/ i >= norm_length) /\ i<length a) ==> (get h2 a i == get h1 a i))) *)
+(*       // Conditions from fdifference_aux_1 *)
+(*       /\ (forall (i:nat). *)
+(* 	  ((i >= ctr+1 /\ i < norm_length) ==> *)
+(* 	    v (get h1 b i) >= v (get h1 a i) /\ get h1 a i == get h0 a i) *)
+(* 	  /\ (((i<ctr \/ i >= norm_length) /\ i<length a) ==> get h1 a i == get h0 a i)) *)
+(*       /\ v (get h1 a ctr) = v (get h0 b ctr) - v (get h0 a ctr))) *)
+(*     (ensures ( *)
+(*       (live h0 a) /\ (live h0 b) /\ (live h2 a) /\ (live h2 b) *)
+(*       /\ (modifies_1 a h0 h2) *)
+(*       /\ (length a = length a) *)
+(*       /\ (forall (i:nat). (i>= ctr /\ i<norm_length) ==> (v (get h2 a i) = v (get h0 b i) - v (get h0 a i))) *)
+(*       )) *)
+      
+(* let fdifference_aux_2_0 h0 h1 h2 a b ctr = *)
+(*   //@@ *)
+(*   (\* no_upd_lemma h0 h1 b ((only a)); *\) *)
+(*   assert(length a = length a); *)
+(*   assert(forall (i:nat). (i>= ctr+1 /\ i<norm_length) ==> *)
+(* 	  (v (get h2 a i) = v (get h1 b i) - v (get h1 a i)));   *)
+(*   assert(forall (i:nat). (i>=ctr+1 /\ i < norm_length) ==> get h1 a i == get h0 a i);  *)
+(*   assert(get h2 a ctr == get h1 a ctr);  *)
+(*   assert(v (get h1 a ctr) = v (get h0 b ctr) - v (get h0 a ctr)); *)
+(*   cut(forall (i:nat). (i>= ctr+1 /\ i<norm_length) ==> *)
+(* 	  (v (get h2 a i) = v (get h0 b i) - v (get h0 a i)));  *)
+(*   cut(True /\ v (get h2 a ctr) = v (get h0 b ctr) - v (get h0 a ctr));  *)
+(*   (\* FdifferenceLemmas.helper_lemma_5 ctr norm_length; *\) *)
+(*   assert(forall (i:nat). (i>=ctr /\ i < norm_length) ==> *)
+(* 	   (v (get h2 a i) = v (get h0 b i) - v (get h0 a i))) *)
+
+(* (\* #reset-options *\) *)
+
+(* val fdifference_aux_2_1: h0:heap -> h1:heap -> h2:heap -> a:bigint -> b:bigint{disjoint a b} ->  *)
+(*   ctr:nat{ctr < norm_length} -> *)
+(*   Lemma  *)
+(*     (requires ( *)
+(*       live h0 a /\ live h1 a /\ live h2 a /\ live h0 b /\ live h1 b /\ live h2 b *)
+(*       /\ modifies_1 a h0 h1 /\ modifies_1 a h1 h2 *)
+(*       /\ length a = length a /\ length a = length a *)
+(*       /\ length b = length b /\ length b = length b *)
+(*       /\ (norm_length <= length a /\ norm_length <= length b) *)
+(*       // Conditions from fdifference_aux *)
+(*       /\ (modifies_1 a h1 h2) *)
+(*       /\ (forall (i:nat). *)
+(* 	  ((i>=ctr+1 /\ i<norm_length) ==> (v (get h2 a i) = v (get h1 b i) - v (get h1 a i))) *)
+(* 	  /\ (((i<ctr+1 \/ i >= norm_length) /\ i<length a) ==> (get h2 a i == get h1 a i))) *)
+(*       // Conditions from fdifference_aux_1 *)
+(*       /\ (forall (i:nat). *)
+(* 	  ((i >= ctr+1 /\ i < norm_length) ==> *)
+(* 	    v (get h1 b i) >= v (get h1 a i) /\ get h1 a i == get h0 a i) *)
+(* 	  /\ (((i<ctr \/ i >= norm_length) /\ i<length a) ==> get h1 a i == get h0 a i)) *)
+(*       /\ v (get h1 a ctr) = v (get h0 b ctr) - v (get h0 a ctr))) *)
+(*     (ensures ( *)
+(*       (live h0 a) /\ (live h0 b) /\ (live h2 a) /\ (live h2 b) *)
+(*       /\ (norm_length <= length a /\ norm_length <= length b) *)
+(*       /\ (modifies_1 a h0 h2) *)
+(*       /\ (length a = length a) *)
+(*       /\ (forall (i:nat). ((i<ctr \/ i >= norm_length) /\ i<length a) ==> (get h2 a i == get h0 a i)) *)
+(*     )) *)
+(* let fdifference_aux_2_1 h0 h1 h2 a b ctr =  *)
+(*   //@@ *)
 (*   () *)
 
-(* #reset-options *)
+(* val fdifference_aux_2: h0:heap -> h1:heap -> h2:heap -> a:bigint -> b:bigint{disjoint a b} ->  *)
+(*   ctr:nat{ctr < norm_length} -> Lemma *)
+(*     (requires ( *)
+(*       live h0 a /\ live h1 a /\ live h2 a /\ live h0 b /\ live h1 b /\ live h2 b *)
+(*       /\ modifies_1 a h0 h1 /\ modifies_1 a h1 h2 *)
+(*       /\ length a = length a /\ length a = length a *)
+(*       /\ length b = length b /\ length b = length b *)
+(*       /\ (norm_length <= length a /\ norm_length <= length b) *)
+(*       // Conditions from fdifference_aux *)
+(*       /\ (modifies_1 a h1 h2) *)
+(*       /\ (forall (i:nat).  *)
+(* 	  ((i>= ctr+1 /\ i<norm_length) ==> *)
+(* 	    (v (get h2 a i) = v (get h1 b i) - v (get h1 a i))) *)
+(* 	  /\ (((i<ctr+1 \/ i >= norm_length) /\ i<length a) ==> (get h2 a i == get h1 a i))) *)
+(*       // Conditions from fdifference_aux_1 *)
+(*       /\ (forall (i:nat). *)
+(* 	  ((i >= ctr+1 /\ i < norm_length) ==> v (get h1 b i) >= v (get h1 a i) *)
+(* 						/\ get h1 a i == get h0 a i) *)
+(* 	  /\ (((i<ctr \/ i >= norm_length) /\ i<length a) ==> get h1 a i == get h0 a i)) *)
+(*       /\ v (get h1 a ctr) = v (get h0 b ctr) - v (get h0 a ctr))) *)
+(*     (ensures ( *)
+(*       (live h0 a) /\ (live h0 b) /\ (live h2 a) /\ (live h2 b) *)
+(*       /\ (norm_length <= length a /\ norm_length <= length b) *)
+(*       /\ (modifies_1 a h0 h2) *)
+(*       /\ (length a = length a) *)
+(*       /\ (forall (i:nat). *)
+(* 	  ((i>= ctr /\ i<norm_length) ==>  *)
+(* 	    (v (get h2 a i) = v (get h0 b i) - v (get h0 a i))) *)
+(* 	  /\ (((i<ctr \/ i >= norm_length) /\ i<length a) ==> (get h2 a i == get h0 a i))) *)
+(*       ))       *)
+(* let fdifference_aux_2 h0 h1 h2 a b ctr = *)
+(*   //@@ *)
+(*   fdifference_aux_2_0 h0 h1 h2 a b ctr; *)
+(*   fdifference_aux_2_1 h0 h1 h2 a b ctr *)
 
-val fdifference': a:bigint -> b:bigint{disjoint a b} -> STL unit
-    (requires (fun h -> norm h a /\ filled h b))
-    (ensures (fun h0 u h1 -> norm h0 a /\ filled h0 b /\ filled h1 b /\ live h1 a 
-      /\ modifies_1 a h0 h1
-      /\ eval h1 a norm_length = eval h0 b norm_length - eval h0 a norm_length
-      /\ (forall (i:nat). i < norm_length ==> v (get h1 a i) = v (get h0 b i) - v (get h0 a i))  ))
-let fdifference' a b =
-  //@@
-  let h0 = HST.get() in
-  auxiliary_lemma_0 h0 a h0 b; 
-  fdifference_aux a b 0ul; 
-  let h1 = HST.get() in
-  (* auxiliary_lemma_1 h0 h1 ((only a)) min max b ;  *)
-  subtraction_lemma h0 h1 a b norm_length
+(* (\* #reset-options *\) *)
+
+(* val fdifference_aux: a:bigint -> b:bigint{disjoint a b} -> ctr:u32{U32.v ctr <= norm_length } -> STL unit *)
+(*     (requires (fun h -> live h a /\ live h b *)
+(*       /\ (forall (i:nat). (i >= U32.v ctr /\ i < norm_length) ==> (v (get h b i) >= v (get h a i))) )) *)
+(*     (ensures (fun h0 _ h1 ->  *)
+(*       (live h0 a) /\ (live h0 b) /\ (live h1 a) /\ (live h1 b) *)
+(*       /\ (norm_length <= length a /\ norm_length <= length b) *)
+(*       /\ (modifies_1 a h0 h1) *)
+(*       /\ (length a = length a) *)
+(*       /\ (forall (i:nat).  *)
+(* 	  ((i>= U32.v ctr /\ i<norm_length) ==>   *)
+(* 	    (v (get h1 a i) = v (get h0 b i) - v (get h0 a i))) *)
+(* 	  /\ (((i<U32.v ctr \/ i >= norm_length) /\ i<length a) ==> (get h1 a i == get h0 a i))) *)
+(*     )) *)
+(* let rec fdifference_aux a b ctr = *)
+(*   //@@ *)
+(*   let h0 = HST.get() in *)
+(*   if U32.eq ctr nlength then () *)
+(*   else begin *)
+(*       fdifference_aux_1 a b ctr;  *)
+(*       let h1 = HST.get() in *)
+(*       (\* no_upd_lemma h0 h1 b ((only a)); *\) *)
+(*       fdifference_aux a b (ctr+|1ul);  *)
+(*       let h2 = HST.get() in *)
+(*       fdifference_aux_2 h0 h1 h2 a b (U32.v ctr) *)
+(*   end *)
+  
+(* (\* #reset-options *\) *)
+
+(* val subtraction_lemma_aux: h0:heap ->  h1:heap -> a:bigint{live h0 a /\ live h1 a} ->  *)
+(*   b:bigint{live h0 b} -> len:pos{len <= length a /\ len <= length b *)
+(*     /\ (forall (i:nat). i < len ==> v (get h1 a i) = v (get h0 b i) - v (get h0 a i)) } -> *)
+(*   Lemma (requires ( (eval h0 b (len-1) - eval h0 a (len-1) = eval h1 a (len-1)) *)
+(* 		/\ (v (get h1 a (len-1)) = v (get h0 b (len-1)) - v (get h0 a (len-1))) ) ) *)
+(*     (ensures (eval h0 b len - eval h0 a len = eval h1 a len)) *)
+(* let subtraction_lemma_aux h0 h1 a b len = *)
+(*   //@@ *)
+(*   eval_def h1 a len; *)
+(*   assert(eval h1 a len = pow2 (bitweight (templ) (len-1)) * v (get h1 a (len-1)) + eval h1 a (len-1)); *)
+(*   assert(v (get h1 a (len-1)) = v (get h0 b (len-1)) - v (get h0 a (len-1)));  *)
+(*   Math.Axioms.distributivity_sub_right (pow2 (bitweight (templ) (len-1))) (v (get h0 b (len-1)))  (v (get h0 a (len-1)));  *)
+(*   assert(eval h1 a len = (pow2 (bitweight (templ) (len-1)) * v (get h0 b (len-1)) - pow2 (bitweight (templ) (len-1)) * v (get h0 a (len-1))) + eval h1 a (len-1)); *)
+(*   (\* FdifferenceLemmas.helper_lemma_2  *\) *)
+(*   (\* 		(pow2 (bitweight (templ) (len-1)) * v (get h0 b (len-1))) *\) *)
+(*   (\* 		(pow2 (bitweight (templ) (len-1)) * v (get h0 a (len-1))) *\) *)
+(*   (\* 		(eval h0 b (len-1)) *\) *)
+(*   (\* 		(eval h0 a (len-1)); *\) *)
+(*   eval_def h0 a len; *)
+(*   eval_def h0 b len *)
+
+(* (\* #reset-options *\) *)
+
+(* val subtraction_lemma: *)
+(*   h0:heap -> h1:heap -> a:bigint{live h0 a /\ live h1 a} -> b:bigint{live h0 b} -> *)
+(*   len:nat{len <= length a /\ len <= length b *)
+(*   /\ (forall (i:nat). i < len ==> v (get h1 a i) = v (get h0 b i) - v (get h0 a i)) } -> Lemma *)
+(*     (requires (True)) *)
+(*     (ensures ( eval h0 b len - eval h0 a len = eval h1 a len )) *)
+(* let rec subtraction_lemma h0 h1 a b len = *)
+(*   //@@ *)
+(*   match len with *)
+(*   | 0 -> () *)
+(*   | _ -> subtraction_lemma h0 h1 a b (len-1); *)
+(*     subtraction_lemma_aux h0 h1 a b len *)
+
+(* (\* #reset-options *\) *)
+
+(* val subtraction_max_value_lemma: h0:heap -> h1:heap -> a:bigint{live h0 a} ->  *)
+(*   b:bigint{live h0 b /\ length a = length b} -> *)
+(*   c:bigint{live h1 c /\ length c = length a *)
+(*    /\ (forall (i:nat). (i<length c) ==> v (get h1 c i) = v (get h0 b i) - v (get h0 a i)) } -> *)
+(*   Lemma *)
+(*     (requires (True)) *)
+(*     (ensures (maxValue h1 c (length c) <= maxValue h0 b (length c))) *)
+(* let subtraction_max_value_lemma h0 h1 a b c =  *)
+(*   //@@ *)
+(*   () *)
+
+(* (\* #reset-options *\) *)
+
+(* val max_value_lemma: h:heap -> a:bigint{live h a} -> m:nat ->Lemma  *)
+(*     (requires (forall (n:nat). n < length a ==> v (get h a n) <= m)) *)
+(*     (ensures (maxValue h a (length a) <= m)) *)
+(* let max_value_lemma h a m =  *)
+(*   //@@ *)
+(*   () *)
+
+(* val subtraction_max_value_lemma_extended: h0:heap -> h1:heap -> a:bigint{live h0 a} ->  *)
+(*   b:bigint{live h0 b} -> *)
+(*   c:bigint{live h1 c /\ length a = length c} ->  *)
+(*   Lemma *)
+(*     (requires ((forall (i:nat). (i<norm_length) ==>  *)
+(* 		  v (get h1 c i) = v (get h0 b i) - v (get h0 a i)) *)
+(* 	       /\ (forall (i:nat). (i < length c /\ i >= norm_length) ==> *)
+(* 		   v (get h1 c i) = v (get h0 a i)))) *)
+(*     (ensures (maxValue h1 c (length c) <= max (maxValue h0 a (length a)) (maxValue h0 b (length b)))) *)
+(* let subtraction_max_value_lemma_extended h0 h1 a b c =  *)
+(*   //@@ *)
+(*   cut ( forall (i:nat). (i < length c /\ i >= norm_length) *)
+(* 	==> (v (get h1 c i) = v (get h0 a i) /\ v (get h1 c i) <= maxValue h0 a (length a))); *)
+(*   cut ( forall (i:nat). (i < length c /\ i >= norm_length) *)
+(*   	==> v (get h1 c i) <= max (maxValue h0 a (length a)) (maxValue h0 b (length b)));	 *)
+(*   assert ( forall (i:nat). (i < norm_length) *)
+(* 	==> v (get h1 c i) = v (get h0 b i) - v (get h0 a i)); *)
+(*   (\* assert(forall (i:nat). (i < norm_length) ==> v (get h1 c i) = v (get h0 b i) - v (get h0 a i) ==> v (get h1 c i) <= v (get h0 b i) ==> v (get h1 c i) <= maxValue h0 b);  *\) *)
+(*   (\* cut ( forall (i:nat). (i < norm_length) *\) *)
+(*   (\* 	==> v (get h1 c i) <= maxValue h0 b);  *\) *)
+(*   (\* cut ( forall (i:nat). (i < norm_length) *\) *)
+(*   (\* 	==> (v (get h0 a i) <= maxValue h0 a /\ v (get h0 b i) <= maxValue h0 b));  *\) *)
+(*   cut ( forall (i:nat). (i < norm_length) *)
+(* 	==> v (get h1 c i) <= max (maxValue h0 a (length a)) (maxValue h0 b (length b))) *)
+
+(* (\* #reset-options *\) *)
+
+(* val auxiliary_lemma_2: ha:heap -> a:bigint{norm ha a} -> hb:heap -> b:bigint{filled hb b} ->  *)
+(*   i:nat{i < norm_length} -> Lemma (v (get hb b i) - v (get ha a i) < pow2 (templ i + 1)) *)
+(* let auxiliary_lemma_2 ha a hb b i = () *)
+(*   //@@ *)
+(*   (\* assert(True /\ bitsize (v (get hb b i)) max);  *\) *)
+(*   (\* Lemmas.pow2_increases_2 min (templ i);  *\) *)
+(*   (\* assert(bitsize (v (get ha a i)) (templ i));  *\) *)
+(*   (\* assert(v (get ha a i) < pow2 (templ i));  *\) *)
+(*   (\* cut(True /\ v (get ha a i) < pow2 min);  *\) *)
+(*   (\* assert(bitsize (v (get ha a i)) min);  *\) *)
+(*   (\* UInt.sub_lemma #max (v (get hb b i)) (v (get ha a i)) *\) *)
+
+(* (\* #reset-options *\) *)
+
+(* val auxiliary_lemma_0: ha:heap -> a:bigint{norm ha a} -> hb:heap -> b:bigint{filled hb b} -> *)
+(*   Lemma (forall (i:nat). i < norm_length ==> v (get hb b i) - v (get ha a i) < pow2 (templ i + 1)) *)
+(* let auxiliary_lemma_0 ha a hb b =  *)
+(*   //@@ *)
+(*   () *)
+
+(* (\* #reset-options *\) *)
+
+(* (\* val auxiliary_lemma_1: h0:heap -> h1:heap -> mods:FStar.Set.set abuffer -> b:bigint{filled h0 b} -> *\) *)
+(* (\*   Lemma (requires (live h1 b /\ modifies mods h0 h1 /\ not(FStar.Set.mem (Ref (getRef b)) mods))) *\) *)
+(* (\* 	(ensures (filled h1 b)) *\) *)
+(* (\* let auxiliary_lemma_1 h0 h1 mods min max b =  *\) *)
+(* (\*   //@@ *\) *)
+(* (\*   assert(FStar.Seq.Eq (sel h0 (getRef b)) (sel h1 (getRef b)));  *\) *)
+(* (\*   () *\) *)
+
+(* (\* #reset-options *\) *)
+
+(* val fdifference': a:bigint -> b:bigint{disjoint a b} -> STL unit *)
+(*     (requires (fun h -> norm h a /\ filled h b)) *)
+(*     (ensures (fun h0 u h1 -> norm h0 a /\ filled h0 b /\ filled h1 b /\ live h1 a  *)
+(*       /\ modifies_1 a h0 h1 *)
+(*       /\ eval h1 a norm_length = eval h0 b norm_length - eval h0 a norm_length *)
+(*       /\ (forall (i:nat). i < norm_length ==> v (get h1 a i) = v (get h0 b i) - v (get h0 a i))  )) *)
+(* let fdifference' a b = *)
+(*   //@@ *)
+(*   let h0 = HST.get() in *)
+(*   auxiliary_lemma_0 h0 a h0 b;  *)
+(*   fdifference_aux a b 0ul;  *)
+(*   let h1 = HST.get() in *)
+(*   (\* auxiliary_lemma_1 h0 h1 ((only a)) min max b ;  *\) *)
+(*   subtraction_lemma h0 h1 a b norm_length *)
 
 
