crypto_hst/ec/Hacl.EC.Curve25519.Bignum.Fdifference.fst
@@ -4,13 +4,15 @@ open FStar.Mul
 open FStar.HST
 open FStar.HyperStack
 open FStar.Ghost
-open Hacl.UInt64
-(* open Hacl.SBuffer *)
 open FStar.Buffer
 open FStar.Math.Lib
+
+open Hacl.UInt64
+
 open Hacl.EC.Curve25519.Parameters
 open Hacl.EC.Curve25519.Bigint
-
+open Hacl.EC.Curve25519.Utils
+open Hacl.EC.Curve25519.Bignum.Fdifference.Lemmas
 
 #reset-options "--initial_fuel 0 --max_fuel 0"
 
@@ -23,6 +25,43 @@ module U32 = FStar.UInt32
 module H8  = Hacl.UInt8
 module H32  = Hacl.UInt32
 module H64  = Hacl.UInt64
+
+
+val add_big_zero_core:
+  b:bigint ->
+  Stack unit
+    (requires (fun h -> norm h b))
+    (ensures (fun h0 _ h1 -> addedZero h0 h1 b /\ modifies_1 b h0 h1))
+let add_big_zero_core b =
+  let two52m38 = (Hacl.Cast.uint64_to_sint64 0xfffffffffffdauL) in // pow2 52 - 38
+  let two52m2 =  (Hacl.Cast.uint64_to_sint64 0xffffffffffffeuL) in // pow2 52 - 2
+  lemma_pow2_52m38 ();
+  lemma_pow2_52m2 ();
+  cut(v two52m38 = pow2 52 - 38 /\ v two52m2 = pow2 52 - 2);
+  let b0 = b.(0ul) in
+  let b1 = b.(1ul) in
+  let b2 = b.(2ul) in
+  let b3 = b.(3ul) in
+  let b4 = b.(4ul) in
+  lemma_add_big_zero_core b0 b1 b2 b3 b4;
+  let c0 = b0 +^ two52m38 in
+  let c1 = b1 +^ two52m2  in
+  let c2 = b2 +^ two52m2  in
+  let c3 = b3 +^ two52m2  in
+  let c4 = b4 +^ two52m2  in
+  update_5 b c0 c1 c2 c3 c4
+
+
+(*
+val add_big_zero: b:bigint -> Stack unit
+  (requires (fun h -> live h b))
+  (ensures (fun h0 _ h1 -> live h1 b /\ modifies_1 b h0 h1))
+let add_big_zero b =
+  (* let h0 = HST.get() in *)
+  add_big_zero_core b(* ; *)
+  (* let h1 = HST.get() in *)
+  (* add_big_zero_lemma h0 h1 b *)
+
 
 (* #reset-options *)
 val fdifference_aux_1:
