crypto_hst/ec/Hacl.EC.Curve25519.Bignum.Fsum.Lemmas.fst
@@ -1,261 +1,83 @@
-module Hacl.EC.Curve25519.Bignum.Fsum
+module Hacl.EC.Curve25519.Bignum.Fsum.Lemmas
 
 open FStar.Mul
 open FStar.HST
 open FStar.HyperStack
 open FStar.Ghost
-open Hacl.UInt64
-open Hacl.SBuffer
+open FStar.Buffer
 open FStar.Math.Lib
+open FStar.Math.Lemmas
+
+open Hacl.UInt64
+
 open Hacl.EC.Curve25519.Parameters
 open Hacl.EC.Curve25519.Bigint
+open Hacl.EC.Curve25519.Bignum.Lemmas.Utils
+
+module U32 = FStar.UInt32
+module H64 = Hacl.UInt64
 
 #reset-options "--initial_fuel 0 --max_fuel 0"
 
-module U32 = FStar.UInt32
 
-abstract type willNotOverflow (h:heap) 
-		     (a:bigint{live h a /\ length a >= norm_length}) 
-		     (b:bigint{live h b /\ length b >= norm_length}) 
-		     (ctr:nat) =
-  (forall (i:nat). {:pattern (v (get h a i) + v (get h b i))} (i >= ctr /\ i < norm_length) ==> v (get h a i) + v (get h b i) < pow2 platform_size)
+let willNotOverflow (h:heap) (a:bigint) (b:bigint) : GTot Type0 =
+  live h a /\ live h b /\ length a >= norm_length /\ length b >= norm_length
+  /\ v (get h a 0) + v (get h b 0) < pow2 64
+  /\ v (get h a 1) + v (get h b 1) < pow2 64
+  /\ v (get h a 2) + v (get h b 2) < pow2 64
+  /\ v (get h a 3) + v (get h b 3) < pow2 64
+  /\ v (get h a 4) + v (get h b 4) < pow2 64
 
-abstract type notModified (h0:heap) (h1:heap) 
-			(a:bigint{live h0 a /\ live h1 a /\ length a >= norm_length})
-			(ctr:nat) =
-  (forall (i:nat). {:pattern (get h1 a i)}
-    ((i <> ctr /\ i < length a) ==>  get h1 a i = get h0 a i))
+let isSum (h:heap) (h1:heap) (a:bigint) (b:bigint) : GTot Type0 =
+  live h a /\ live h1 a /\ live h b /\ length a >= norm_length /\ length b >= norm_length
+  /\ v (get h a 0) + v (get h b 0) = v (get h1 a 0)
+  /\ v (get h a 1) + v (get h b 1) = v (get h1 a 1)
+  /\ v (get h a 2) + v (get h b 2) = v (get h1 a 2)
+  /\ v (get h a 3) + v (get h b 3) = v (get h1 a 3)
+  /\ v (get h a 4) + v (get h b 4) = v (get h1 a 4)
 
-(* val fsum_index_aux: *)
-(*   a:bigint -> b:bigint{disjoint a b} -> ctr:u32{U32.v ctr < norm_length} -> *)
-(*   STL unit *)
-(*     (requires (fun h ->  *)
-(*       live h a /\ live h b /\ norm_length <= length a /\ norm_length <= length b *)
-(*       /\ willNotOverflow h a b (U32.v ctr) )) *)
-(*     (ensures (fun h0 _ h1 ->  *)
-(*       let ctr = U32.v ctr in *)
-(*       live h0 a /\ live h1 a /\ live h0 b /\ live h1 b *)
-(*       /\ length a = length a /\ length b = length b *)
-(*       /\ norm_length <= length a /\ norm_length <= length b /\ modifies_1 a h0 h1 *)
-(*       /\ (willNotOverflow h1 a b (ctr+1)) *)
-(*       /\ (notModified h0 h1 a (ctr)) *)
-(*       /\ v (get h1 a (ctr)) = v (get h0 a ctr) + v (get h0 b ctr))) *)
-(* let fsum_index_aux a b ctr = *)
-(*   //@@ *)
-(*   let h0 = HST.get() in *)
-(*   let ai = index a ctr in  *)
-(*   let bi = index b ctr in  *)
-(*   assert(U32.v ctr < norm_length);  *)
-(*   assert(b2t(v (get h0 a (U32.v ctr)) + v (get h0 b (U32.v ctr)) < pow2 platform_size));  *)
-(*   let z = add ai bi in  *)
-(*   upd a ctr z;  *)
-(*   let h1 = HST.get() in *)
-(*   (\* upd_lemma h0 h1 a ctr z;  *\) *)
-(*   assert(v (get h1 a (U32.v ctr)) = v (get h0 a (U32.v ctr)) + v (get h0 b (U32.v ctr)));  *)
-(*   assert(notModified h0 h1 a (U32.v ctr));  *)
-(*   assert(willNotOverflow h1 a b ((U32.v ctr)+1)); *)
-(*   (\* no_upd_lemma h0 h1 b (only a) *\) *)
-(*   () *)
+let bound52 (h:heap) (b:bigint) : GTot Type0 =
+  live h b /\ length b >= norm_length
+  /\ v (get h b 0) < pow2 52
+  /\ v (get h b 1) < pow2 52
+  /\ v (get h b 2) < pow2 52
+  /\ v (get h b 3) < pow2 52
+  /\ v (get h b 4) < pow2 52
 
-abstract let isSum (h0:heap) (h1:heap) (a:bigint{live h0 a /\ live h1 a /\ length a = length a}) 
-		  (b:bigint{live h0 b}) (ctr:nat) =
-  (forall (i:nat). {:pattern (v (get h1 a i))}
-	  (i>=ctr /\ i<norm_length) ==> (v (get h1 a i) = v (get h0 a i) + v (get h0 b i)))
 
-abstract let notModified2 (h0:heap) (h1:heap)
-			 (a:bigint{live h0 a /\ live h1 a})
-			 (ctr:nat) =
-  (forall (i:nat). {:pattern (get h1 a i)} 
-    ((i < ctr \/ i >= norm_length) /\ i < length a) ==> get h1 a i = get h0 a i)
-    
-val fsum_index_lemma: 
-  h0:heap -> h1:heap -> h2:heap -> a:bigint -> b:bigint{disjoint a b} -> ctr:nat{ctr < norm_length} ->
+let w : U32.t -> Tot int = U32.v
+
+#reset-options "--z3timeout 5 --initial_fuel 0 --max_fuel 0"
+
+val lemma_fsum_0:
+  a0:H64.t -> a1:H64.t -> a2:H64.t -> a3:H64.t -> a4:H64.t ->
+  b0:H64.t -> b1:H64.t -> b2:H64.t -> b3:H64.t -> b4:H64.t ->
   Lemma (requires (
-      live h0 a /\ live h1 a /\ live h2 a /\ live h0 b /\ live h1 b /\ live h2 b
-      /\ modifies_1 a h0 h1 /\ modifies_1 a h1 h2
-      /\ modifies_1 a h1 h2
-      /\ notModified2 h1 h2 a (ctr+1)
-      /\ isSum h1 h2 a b (ctr+1)
-      /\ willNotOverflow h0 a b (ctr+1)
-      /\ notModified h0 h1 a ctr
-      /\ v (get h1 a ctr) = v (get h0 a ctr) + v (get h0 b ctr) ))
-    (ensures (
-      live h0 a /\ live h0 b /\ live h2 a /\ live h2 b
-      /\ modifies_1 a h0 h2
-      /\ isSum h0 h2 a b ctr ))
-let fsum_index_lemma h0 h1 h2 a b ctr =
-  //@@
-  (* no_upd_lemma h0 h1 b (only a); *)
-  (* no_upd_lemma h1 h2 b (only a); *)
-  assert(isSum h1 h2 a b (ctr+1)); 
-  assert(notModified2 h1 h2 a (ctr+1)); 
-  assert(notModified h0 h1 a ctr); 
-  cut(isSum h0 h2 a b (ctr+1)); 
-  cut(True /\ v (get h2 a ctr) = v (get h0 a ctr) + v (get h0 b ctr)); 
-  (* FsumLemmas.auxiliary_lemma_7 ctr norm_length;  *)
-  assert(isSum h0 h2 a b ctr)
+	  v a0 < pow2 51 /\ v a1 < pow2 51 /\ v a2 < pow2 51 /\ v a3 < pow2 51 /\ v a4 < pow2 51
+	  /\ v b0 < pow2 51 /\ v b1 < pow2 51 /\ v b2 < pow2 51 /\ v b3 < pow2 51 /\ v b4 < pow2 51))
+	(ensures  (
+		  v a0 + v b0 < pow2 64 /\ v a1 + v b1 < pow2 64 /\ v a2 + v b2 < pow2 64
+		  /\ v a3 + v b3 < pow2 64 /\ v a4 + v b4 < pow2 64))
+let lemma_fsum_0 a0 a1 a2 a3 a4 b0 b1 b2 b3 b4 =
+  pow2_double_sum 51;
+  pow2_lt_compat 64 52
 
-(* // Verified, try with big timeout *)
-(* val fsum_index: *)
-(*   a:bigint -> b:bigint{disjoint a b} -> ctr:u32{U32.v ctr <= norm_length } -> *)
-(*   STL unit *)
-(*     (requires (fun h -> live h a /\ live h b *)
-(*       /\ (forall (i:nat). (i >= U32.v ctr /\ i < norm_length) ==> *)
-(* 	  (v (get h a i) + v (get h b i) < pow2 platform_size)) )) *)
-(*     (ensures (fun h0 _ h1 -> let ctr = U32.v ctr in *)
-(*       live h0 a /\ live h0 b /\ live h1 a /\ live h1 b *)
-(*       /\ modifies_1 a h0 h1 *)
-(*       /\ isSum h0 h1 a b ctr *)
-(*       /\ notModified2 h0 h1 a ctr )) *)
-(* let rec fsum_index a b ctr = *)
-(*   //@@ *)
-(*   let h0 = HST.get() in *)
-(*   if U32.eq nlength ctr then () *)
-(*   else ( *)
-(*     fsum_index_aux a b ctr;  *)
-(*     let h1 = HST.get() in *)
-(*     (\* no_upd_lemma h0 h1 b (only a);  *\) *)
-(*     (\* FsumLemmas.auxiliary_lemma_6 norm_length ctr;  *\) *)
-(*     fsum_index a b (U32.add ctr 1ul);  *)
-(*     let h2 = HST.get() in *)
-(*     fsum_index_lemma h0 h1 h2 a b (U32.v ctr) *)
-(*   ) *)
-  
-(* #reset-options *)
+#reset-options "--z3timeout 5 --initial_fuel 0 --max_fuel 0"
 
-val addition_lemma_aux: h0:heap ->  h1:heap -> a:bigint{live h0 a /\ live h1 a} -> 
-  b:bigint{live h0 b} -> len:pos{len <= length a /\ len <= length b
-	   /\ (forall (i:nat). i < len ==> v (get h1 a i) = v (get h0 a i) + v (get h0 b i)) } ->
-  Lemma
-    (requires ( (eval h0 a (len-1) + eval h0 b (len-1) = eval h1 a (len-1))
-		/\ (v (get h1 a (len-1)) = v (get h0 a (len-1)) + v (get h0 b (len-1))) ) )
-    (ensures (eval h0 a len + eval h0 b len = eval h1 a len))
-let addition_lemma_aux h0 h1 a b len =
-  eval_def h1 a len;
-  assert(eval h1 a len = pow2 (bitweight templ (len-1)) * v (get h1 a (len-1)) + eval h1 a (len-1));
-  assert(v (get h1 a (len-1)) = v (get h0 a (len-1)) + v (get h0 b (len-1)));
-  Math.Axioms.distributivity_add_right (pow2 (bitweight templ (len-1))) (v (get h0 a (len-1)))  (v (get h0 b (len-1))); 
-  assert(eval h1 a len = (pow2 (bitweight (templ) (len-1)) * v (get h0 a (len-1)) + pow2 (bitweight (templ) (len-1)) * v (get h0 b (len-1))) + eval h1 a (len-1));
-  (* FsumLemmas.helper_lemma_2 (pow2 (bitweight (templ) (len-1)) * v (get h0 a (len-1))) *)
-  (* 		(pow2 (bitweight (templ) (len-1)) * v (get h0 b (len-1))) *)
-  (* 		(eval h0 a (len-1)) *)
-  (* 		(eval h0 b (len-1)); *)
-  eval_def h0 a len;
-  eval_def h0 b len
-
-val addition_lemma: h0:heap -> h1:heap -> a:bigint{live h0 a /\ live h1 a} ->
-  b:bigint{live h0 b} -> len:nat{len <= length a /\ len <= length b /\ len <= length a
-	  /\ (forall (i:nat). i < len ==> v (get h1 a i) = v (get h0 a i) + v (get h0 b i)) } -> Lemma
-    (requires (True))
-    (ensures ( eval h0 a len + eval h0 b len = eval h1 a len ))
-let rec addition_lemma h0 h1 a b len =
-  //@@
-  match len with
-  | 0 -> ()
-  | _ -> addition_lemma h0 h1 a b (len-1);
-    addition_lemma_aux h0 h1 a b len
-
-(* #reset-options *)
-
-val addition_max_value_lemma: h0:heap -> h1:heap -> a:bigint{live h0 a} -> b:bigint{live h0 b /\ length a = length b} -> c:bigint{live h1 c /\ length c = length a 
-  /\ (forall (i:nat{i<length c}). v (get h1 c i) = v (get h0 a i) + v (get h0 b i)) } -> Lemma
-    (requires (True))
-    (ensures (let l = length c in maxValue h1 c l <= maxValue h0 a l + maxValue h0 b l))
-let addition_max_value_lemma h0 h1 a b c = ()
-  
-val max_value_lemma: 
-  h:heap -> a:bigint{ live h a } -> m:nat ->
-  Lemma 
-    (requires (forall (n:nat). n < length a ==> v (get h a n) <= m))
-    (ensures (maxValue h a (length a) <= m))
-let max_value_lemma h a m = ()
-
-(* #reset-options *)
-
-val addition_max_value_lemma_extended: h0:heap -> h1:heap -> a:bigint{live h0 a} -> 
-  b:bigint{live h0 b} -> c:bigint{live h1 c /\ length a = length c} ->
-  idx:nat -> len:nat{len + idx <= length a /\ len <= length b} -> Lemma
-    (requires ((forall (i:nat). {:pattern (v (get h1 c (i+idx)))} 
-		  (i<len) ==> v (get h1 c (i+idx)) = v (get h0 a (i+idx)) + v (get h0 b i))
-	       /\ (forall (i:nat). {:pattern (v (get h1 c i))}
-		   (i < length c /\ (i < idx \/ i >= idx + len)) ==> v (get h1 c i) = v (get h0 a i))))
-    (ensures (maxValue h1 c len <= maxValue h0 a len + maxValue h0 b len))
-let addition_max_value_lemma_extended h0 h1 a b c idx len = 
-  cut ( forall (i:nat). (i < length c /\ (i < idx \/ i >= idx + len))
-	==> (v (get h1 c i) = v (get h0 a i) /\ v (get h1 c i) <= maxValue h0 a len + maxValue h0 b len)); 
-  cut ( forall (i:nat). (i < length c /\ (i < idx \/ i >= idx + len)) 
-  	==> v (get h1 c i) <= maxValue h0 a len + maxValue h0 b len); 
-  cut(forall (i:nat). {:pattern (v (get h1 c i))} (i+idx < idx + len /\ i+idx >= idx) ==> (i >= 0 /\ i < len)); 
-  cut((forall (i:nat). {:pattern (v (get h1 c i))} (i-idx)+idx=i)); 
-  assert(forall (i:nat). {:pattern (v (get h1 c (i)))} (i<len) ==> v (get h1 c (i+idx)) = v (get h0 a (i+idx)) + v (get h0 b i)); 
-  assert(forall (i:nat). {:pattern (v (get h1 c i))} (i >= idx /\ i < idx + len) ==> (v (get h1 c i) = v (get h1 c ((i-idx)+idx)))); 
-  cut ( forall (i:nat). (i < idx + len /\ i >= idx)
-	==> ((v (get h1 c i) = v (get h0 a i) + v (get h0 b (i-idx))) )); 
-  cut ( forall (i:nat). (i < idx + len /\ i >= idx)
-	==> (v (get h0 a i) <= maxValue h0 a len /\ v (get h0 b (i-idx)) <= maxValue h0 b len));
-  cut ( forall (i:nat). (i >= idx /\ i < idx + len)
-	==> v (get h1 c i) <= maxValue h0 a len + maxValue h0 b len);
-  cut ( forall (i:nat). i < length c 
-	==> v (get h1 c i) <= maxValue h0 a len + maxValue h0 b len);
-  max_value_lemma h1 c (maxValue h0 a len + maxValue h0 b len);
-  ()
-
-(* #reset-options *)
-
-val auxiliary_lemma_2: ha:heap -> a:bigint{norm ha a} -> hb:heap -> b:bigint{norm hb b} -> 
-  i:nat{ i < norm_length} -> Lemma
-  (v (get ha a i) + v (get hb b i) < pow2 platform_size)
-let auxiliary_lemma_2 ha a hb b i = ()
-  (* UInt.add_lemma #(templ i) (v (get ha a i)) #(templ i) (v (get hb b i)); *)
-  (* parameters_lemma_0 (); *)
-  (* Lemmas.pow2_increases_2 platform_size (templ i + 1) *)
-
-val auxiliary_lemma_0: 
-  ha:heap -> a:bigint{norm ha a} ->
-  hb:heap -> b:bigint{norm hb b} ->
+val factorization_lemma: unit ->
   Lemma (requires (True))
-	(ensures (forall (i:nat). 
-	  i < norm_length ==> v (get ha a i) + v (get hb b i) < pow2 platform_size))
-let auxiliary_lemma_0 ha a hb b = ()
+	(ensures  (forall a b c. {:pattern (a * (b+c))} a * (b + c) = a * b + a * c))
+let factorization_lemma () = ()
 
-(* #reset-options *)
+#reset-options "--z3timeout 20 --initial_fuel 0 --max_fuel 0"
 
-val auxiliary_lemma_1:
-  h0:heap -> h1:heap -> b:bigint{norm h0 b} ->
-  Lemma (requires (live h1 b /\ Seq.equal (sel h1  b) (sel h0 b)))
-	(ensures (norm h1 b))
-let auxiliary_lemma_1 h0 h1 b = 
-  //@@
-  ()
-
-val auxiliary_lemma_3:
-  h0:heap -> h1:heap -> 
-  a:bigint{norm h0 a /\ live h1 a /\ length a >= norm_length} ->
-  b:bigint{norm h0 b /\ norm h1 b} ->
-  Lemma (requires (forall (i:nat{i>= 0 /\ i<norm_length}). 
-	  (v (get h1 a (i+0)) = v (get h0 a (i+0)) + v (get h0 b (i+0))) ))
-	(ensures (forall (i:nat). i < norm_length ==> v (get h1 a i) = v (get h0 a i) + v (get h0 b i)))
-let auxiliary_lemma_3 h0 h1 a b =	
-  cut (forall (i:nat{ i >= 0 /\ i < norm_length }). True ==> (i < norm_length /\ i+0 = i));
-  cut (forall (i:nat). i < norm_length ==> v (get h1 a i) = v (get h0 a i) + v (get h0 b i))
-
-(* #reset-options *)
-
-(* val fsum': *)
-(*   a:bigint -> b:bigint{disjoint a b} -> STL unit *)
-(*     (requires (fun h -> norm h a /\ norm h b)) *)
-(*     (ensures (fun h0 u h1 -> norm h0 a /\ norm h0 b /\ norm h1 b /\ live h1 a  *)
-(*       /\ modifies_1 a h0 h1 *)
-(*       /\ eval h1 a norm_length = eval h0 a norm_length + eval h0 b norm_length *)
-(*       /\ isSum h0 h1 a b 0 )) *)
-(* let fsum' a b = *)
-(*   let h0 = HST.get() in *)
-(*   auxiliary_lemma_0 h0 a h0 b; *)
-(*   fsum_index a b 0ul; *)
-(*   let h1 = HST.get() in *)
-(*   (\* no_upd_lemma h0 h1 b (only a); *\) *)
-(*   auxiliary_lemma_1 h0 h1 b; *)
-(*   auxiliary_lemma_3 h0 h1 a b; *)
-(*   addition_lemma h0 h1 a b norm_length; *)
-(*   cut(forall (i:nat). (i >= 0 /\ i < norm_length) ==> i < norm_length); *)
-(*   () *)
+val lemma_fsum: h0:mem -> h1:mem -> a:bigint -> b:bigint -> Lemma
+  (requires (norm h0 a /\ norm h0 b /\ isSum h0 h1 a b))
+  (ensures  (norm h0 a /\ norm h0 b /\ isSum h0 h1 a b
+    /\ bound52 h1 a /\ eval h1 a norm_length = eval h0 a norm_length + eval h0 b norm_length))
+let lemma_fsum h0 h1 a b =
+  pow2_double_sum 51;
+  lemma_eval_bigint_5 h0 a;
+  lemma_eval_bigint_5 h0 b;
+  factorization_lemma ();
+  lemma_eval_bigint_5 h1 a
