crypto_hst/ec/Hacl.EC.Curve25519.Bignum.Fsum.fst
@@ -3,13 +3,17 @@ module Hacl.EC.Curve25519.Bignum.Fsum
 open FStar.Mul
 open FStar.HST
 open FStar.HyperStack
+open FStar.Buffer
+open FStar.Buffer.Quantifiers
+(* open Hacl.SBuffer *)
+open FStar.Math.Lib
 open FStar.Ghost
 open Hacl.UInt64
-(* open Hacl.SBuffer *)
-open FStar.Buffer
-open FStar.Math.Lib
+
 open Hacl.EC.Curve25519.Parameters
 open Hacl.EC.Curve25519.Bigint
+open Hacl.EC.Curve25519.Utils
+open Hacl.EC.Curve25519.Bignum.Fsum.Lemmas
 
 #reset-options "--initial_fuel 0 --max_fuel 0"
 
@@ -23,88 +27,49 @@ module H8  = Hacl.UInt8
 module H32  = Hacl.UInt32
 module H64  = Hacl.UInt64
 
-val fsum_index_aux:
+private val fsum_:
   a:bigint ->
   b:bigint{disjoint a b} ->
-  ctr:u32{U32.v ctr < norm_length} ->
   Stack unit
-    (requires (fun h -> live h a /\ live h b /\ norm_length <= length a /\ norm_length <= length b
-      (* /\ willNotOverflow h a b (U32.v ctr) *)
-    ))
-    (ensures (fun h0 _ h1 -> live h1 a /\ modifies_1 a h0 h1
-      (* let ctr = U32.v ctr in *)
-      (* live h0 a /\ live h1 a /\ live h0 b /\ live h1 b *)
-      (* /\ length a = length a /\ length b = length b *)
-      (* /\ norm_length <= length a /\ norm_length <= length b /\ modifies_1 a h0 h1 *)
-      (* /\ (willNotOverflow h1 a b (ctr+1)) *)
-      (* /\ (notModified h0 h1 a (ctr)) *)
-      (* /\ v (get h1 a (ctr)) = v (get h0 a ctr) + v (get h0 b ctr) *)
-    ))
-let fsum_index_aux a b ctr =
-  let ai = a.(ctr) in
-  let bi = b.(ctr) in
-  (* assert(U32.v ctr < norm_length); *)
-  (* assert(b2t(v (get h0 a (U32.v ctr)) + v (get h0 b (U32.v ctr)) < pow2 platform_size));  *)
-  (* let z = ai +^ bi in *)
-  a.(ctr) <- (ai +%^ bi);
-  (* let h1 = HST.get() in *)
-  (* (\* upd_lemma h0 h1 a ctr z;  *\) *)
-  (* assert(v (get h1 a (U32.v ctr)) = v (get h0 a (U32.v ctr)) + v (get h0 b (U32.v ctr)));  *)
-  (* assert(notModified h0 h1 a (U32.v ctr));  *)
-  (* assert(willNotOverflow h1 a b ((U32.v ctr)+1)); *)
-  (* no_upd_lemma h0 h1 b (only a) *)
-  ()
+    (requires (fun h -> norm h a /\ norm h b))
+    (ensures (fun h0 u h1 -> norm h0 a /\ norm h0 b /\ live h1 a /\ modifies_1 a h0 h1
+      /\ isSum h0 h1 a b))
+let fsum_ a b =
+  let h0 = HST.get() in
+  let a0 = a.(0ul) in
+  let a1 = a.(1ul) in
+  let a2 = a.(2ul) in
+  let a3 = a.(3ul) in
+  let a4 = a.(4ul) in
+  let b0 = b.(0ul) in
+  let b1 = b.(1ul) in
+  let b2 = b.(2ul) in
+  let b3 = b.(3ul) in
+  let b4 = b.(4ul) in
+  assert(v a0 = v (get h0 a 0)); assert(v a1 = v (get h0 a 1)); assert(v a2 = v (get h0 a 2));
+  assert(v a3 = v (get h0 a 3)); assert(v a4 = v (get h0 a 4)); assert(v b0 = v (get h0 b 0));
+  assert(v b1 = v (get h0 b 1)); assert(v b2 = v (get h0 b 2)); assert(v b3 = v (get h0 b 3));
+  assert(v b4 = v (get h0 b 4));
+  lemma_fsum_0 a0 a1 a2 a3 a4 b0 b1 b2 b3 b4;
+  let ab0 = a0 +^ b0 in
+  let ab1 = a1 +^ b1 in
+  let ab2 = a2 +^ b2 in
+  let ab3 = a3 +^ b3 in
+  let ab4 = a4 +^ b4 in
+  update_5 a ab0 ab1 ab2 ab3 ab4
 
-val fsum_index:
-  a:bigint ->
-  b:bigint{disjoint a b} ->
-  ctr:u32{U32.v ctr <= norm_length } ->
-  Stack unit
-    (requires (fun h -> live h a /\ live h b
-      (* /\ (forall (i:nat). (i >= U32.v ctr /\ i < norm_length) ==> *)
-      (* 	  (v (get h a i) + v (get h b i) < pow2 platform_size)) *)
-    ))
-    (ensures (fun h0 _ h1 -> live h1 a /\ modifies_1 a h0 h1
-      (* let ctr = U32.v ctr in *)
-      (* live h0 a /\ live h0 b /\ live h1 a /\ live h1 b *)
-      (* /\ modifies_1 a h0 h1 *)
-      (* /\ isSum h0 h1 a b ctr *)
-      (* /\ notModified2 h0 h1 a ctr *)
-    ))
-let rec fsum_index a b ctr =
-  (* //@@ *)
-  (* let h0 = HST.get() in *)
-  if U32 (nlength =^ ctr) then ()
-  else (
-    fsum_index_aux a b ctr;
-    (* let h1 = HST.get() in *)
-    (* no_upd_lemma h0 h1 b (only a);  *)
-    (* FsumLemmas.auxiliary_lemma_6 norm_length ctr;  *)
-    fsum_index a b (U32 (ctr +^ 1ul))
-    (* let h2 = HST.get() in *)
-    (* fsum_index_lemma h0 h1 h2 a b (U32.v ctr) *)
-  )
 
 val fsum':
   a:bigint ->
-  b:bigint{disjoint a b} -> Stack unit
-    (requires (fun h -> live h a /\ live h b
-      (* norm h a /\ norm h b *)
-    ))
-    (ensures (fun h0 u h1 -> live h1 a /\ modifies_1 a h0 h1
-      (* /\ norm h0 a /\ norm h0 b /\ norm h1 b /\ live h1 a *)
-      (* /\ modifies_1 a h0 h1 *)
-      (* /\ eval h1 a norm_length = eval h0 a norm_length + eval h0 b norm_length *)
-      (* /\ isSum h0 h1 a b 0 *)
+  b:bigint{disjoint a b} ->
+  Stack unit
+    (requires (fun h -> norm h a /\ norm h b))
+    (ensures (fun h0 u h1 -> norm h0 a /\ norm h0 b /\ bound52 h1 a /\ modifies_1 a h0 h1
+      /\ isSum h0 h1 a b
+      /\ eval h1 a norm_length = eval h0 a norm_length + eval h0 b norm_length
     ))
 let fsum' a b =
-  (* let h0 = HST.get() in *)
-  (* auxiliary_lemma_0 h0 a h0 b; *)
-  fsum_index a b 0ul
-  (* let h1 = HST.get() in *)
-  (* no_upd_lemma h0 h1 b (only a); *)
-  (* auxiliary_lemma_1 h0 h1 b; *)
-  (* auxiliary_lemma_3 h0 h1 a b; *)
-  (* addition_lemma h0 h1 a b norm_length; *)
-  (* cut(forall (i:nat). (i >= 0 /\ i < norm_length) ==> i < norm_length); *)
-  (* () *)
+  let h0 = HST.get() in
+  fsum_ a b;
+  let h1 = HST.get() in
+  lemma_fsum h0 h1 a b
